theories/backtranslation/cast_help/extract.v
@@ -13,16 +13,16 @@ Definition Ω : expr :=
 Definition Ω_typed Γ τ : (Is_Closed τ) -> (Γ ⊢ₛ Ω : τ).
 Proof.
   intro P.
-  apply App_typed with (τ1 := (TRec (TVar 0 → τ))).
+  apply App_typed with (τ1 := (TRec (TArrow (TVar 0) τ))).
   - apply Lam_typed.
-    apply App_typed with (τ1 := TRec (TVar 0 → τ)).
-    + apply Unfold_typed_help_2 with (τ := (TVar 0 → τ)).
+    apply App_typed with (τ1 := TRec (TArrow (TVar 0) τ)).
+    + apply Unfold_typed_help_2 with (τ := (TArrow (TVar 0) τ)).
       asimpl. by rewrite P. by apply Var_typed.
     + by apply Var_typed.
   - apply Fold_typed. asimpl. rewrite P.
     apply Lam_typed.
-    apply App_typed with (τ1 := TRec (TVar 0 → τ)).
-    + apply Unfold_typed_help_2 with (τ := (TVar 0 → τ)).
+    apply App_typed with (τ1 := TRec (TArrow (TVar 0) τ)).
+    + apply Unfold_typed_help_2 with (τ := (TArrow (TVar 0) τ)).
       asimpl. by rewrite P. by apply Var_typed.
     + by apply Var_typed.
 Qed.
@@ -42,15 +42,15 @@ Definition extract_TUnit : expr :=
             (Ω)
       ).
 
-Definition extract_TUnit_typed Γ : Γ ⊢ₛ extract_TUnit : (Universe → TUnit).
+Definition extract_TUnit_typed Γ : Γ ⊢ₛ extract_TUnit : (TArrow Universe TUnit).
 Proof.
   apply Lam_typed.
-  apply Case_typed with (τ1 := (TUnit + (TVar 0 + TVar 0) + (TVar 0 × TVar 0) + (TVar 0 → TVar 0)).[Universe/]%type)
+  apply Case_typed with (τ1 := (TUnit + (TVar 0 + TVar 0) + (TVar 0 × TVar 0) + (TArrow (TVar 0) (TVar 0))).[Universe/]%type)
                          (τ2 := Universe).
   - eapply Unfold_typed_help_2 with (τ := Universe_body). by asimpl.
     by apply Var_typed.
   - apply Case_typed with (τ1 := (TUnit + (TVar 0 + TVar 0) + (TVar 0 × TVar 0)).[Universe/]%type)
-                          (τ2 := (TVar 0 → TVar 0).[Universe/]%type).
+                          (τ2 := (TArrow (TVar 0) (TVar 0)).[Universe/]%type).
     + by apply Var_typed.
     + eapply Case_typed.
       * by apply Var_typed.
@@ -78,10 +78,10 @@ Definition extract_Ground_TSum : expr :=
             (Ω)
       ).
 
-Definition extract_Ground_TSum_typed Γ : Γ ⊢ₛ extract_Ground_TSum : (Universe → (Universe + Universe))%type.
+Definition extract_Ground_TSum_typed Γ : Γ ⊢ₛ extract_Ground_TSum : (TArrow Universe (Universe + Universe))%type.
 Proof.
   apply Lam_typed.
-  apply Case_typed with (τ1 := (TUnit + (TVar 0 + TVar 0) + (TVar 0 × TVar 0) + (TVar 0 → TVar 0)).[Universe/]%type)
+  apply Case_typed with (τ1 := (TUnit + (TVar 0 + TVar 0) + (TVar 0 × TVar 0) + (TArrow (TVar 0) (TVar 0))).[Universe/]%type)
                          (τ2 := Universe).
   - eapply Unfold_typed_help_2 with (τ := Universe_body). by asimpl. by apply Var_typed.
   - eapply Case_typed. by apply Var_typed.
@@ -108,10 +108,10 @@ Definition extract_Ground_TProd : expr :=
             (Ω)
       ).
 
-Definition extract_Ground_TProd_typed Γ : Γ ⊢ₛ extract_Ground_TProd : (Universe → (Universe × Universe)).
+Definition extract_Ground_TProd_typed Γ : Γ ⊢ₛ extract_Ground_TProd : (TArrow Universe (Universe × Universe)).
 Proof.
   apply Lam_typed.
-  apply Case_typed with (τ1 := (TUnit + (TVar 0 + TVar 0) + (TVar 0 × TVar 0) + (TVar 0 → TVar 0)).[Universe/]%type)
+  apply Case_typed with (τ1 := (TUnit + (TVar 0 + TVar 0) + (TVar 0 × TVar 0) + (TArrow (TVar 0) (TVar 0))).[Universe/]%type)
                          (τ2 := Universe).
   - eapply Unfold_typed_help_2 with (τ := Universe_body). by asimpl. by apply Var_typed.
   - eapply Case_typed. by apply Var_typed.
@@ -132,10 +132,10 @@ Definition extract_Ground_TArrow : expr :=
             (Ω)
       ).
 
-Definition extract_Ground_TArrow_typed Γ : Γ ⊢ₛ extract_Ground_TArrow : (Universe → (Universe → Universe)).
+Definition extract_Ground_TArrow_typed Γ : Γ ⊢ₛ extract_Ground_TArrow : (TArrow Universe (TArrow Universe Universe)).
 Proof.
   apply Lam_typed.
-  apply Case_typed with (τ1 := (TUnit + (TVar 0 + TVar 0) + (TVar 0 × TVar 0) + (TVar 0 → TVar 0)).[Universe/]%type)
+  apply Case_typed with (τ1 := (TUnit + (TVar 0 + TVar 0) + (TVar 0 × TVar 0) + (TArrow (TVar 0) (TVar 0))).[Universe/]%type)
                          (τ2 := Universe).
   - eapply Unfold_typed_help_2 with (τ := Universe_body). by asimpl. by apply Var_typed.
   - eapply Case_typed. by apply Var_typed.
@@ -150,10 +150,10 @@ Definition extract_Ground_TRec : expr :=
             (Fold (Var 0))
       ).
 
-Definition extract_Ground_TRec_typed Γ : Γ ⊢ₛ extract_Ground_TRec : (Universe → TRec Universe).
+Definition extract_Ground_TRec_typed Γ : Γ ⊢ₛ extract_Ground_TRec : (TArrow Universe (TRec Universe)).
 Proof.
   apply Lam_typed.
-  apply Case_typed with (τ1 := (TUnit + (TVar 0 + TVar 0) + (TVar 0 × TVar 0) + (TVar 0 → TVar 0)).[Universe/]%type)
+  apply Case_typed with (τ1 := (TUnit + (TVar 0 + TVar 0) + (TVar 0 × TVar 0) + (TArrow (TVar 0) (TVar 0))).[Universe/]%type)
                          (τ2 := Universe).
   - eapply Unfold_typed_help_2 with (τ := Universe_body). by asimpl. by apply Var_typed.
   - by apply Ω_typed.
@@ -170,7 +170,7 @@ Definition extract (τ : cast_calculus.types.type) (G : Ground τ) : expr :=
   end.
 
 Lemma extract_typed {τG : cast_calculus.types.type} {G : Ground τG} Γ :
-  Γ ⊢ₛ (extract τG G) : (Universe → <<τG>>).
+  Γ ⊢ₛ (extract τG G) : (TArrow Universe <<τG>>).
 Proof.
   destruct G.
     + apply extract_TUnit_typed.
