theories/backtranslation/cast_help/general.v
@@ -6,35 +6,42 @@ From fae_gtlc_mu.backtranslation.cast_help Require Export universe embed extract
 (** emulation of a cast between an arbitrary pair of consistent types *)
 (* recursively defined on the alternative consistency relation *)
 
-Fixpoint 𝓕 (A : list (types.type * types.type)) (τi τf : cast_calculus.types.type) (P : A ⊢ τi ~ τf) : expr :=
+Fixpoint 𝓕 {A : list (types.type * types.type)} {τi τf : cast_calculus.types.type} (P : A ⊢ τi ~ τf) : expr :=
   match P with
   | consStarTGround _ τG G => extract τG G
   | consTGroundStar _ τG G => embed τG G
   | consTauStar _ τ τG pUBτ pτnG pτnStar pτSτG pτConsτG =>
     factorization_up
-      (𝓕 A τ τG pτConsτG) τG (get_shape_is_ground pτSτG)
+      (𝓕 pτConsτG) τG (get_shape_is_ground pτSτG)
   | consStarTau _ τ τG pUBτ pτnG pτnStar pτSτG pτGConsτ =>
     factorization_down
-      (𝓕 A τG τ pτGConsτ) τG (get_shape_is_ground pτSτG)
+      (𝓕 pτGConsτ) τG (get_shape_is_ground pτSτG)
   | consBaseBase _ => identity
   | consStarStar _ => identity
   | consTSumTSum _ τ1 τ1' τ2 τ2' pCons1 pCons2 =>
     between_TSum
-      (𝓕 A τ1 τ1' pCons1)
-      (𝓕 A τ2 τ2' pCons2)
+      (𝓕 pCons1)
+      (𝓕 pCons2)
   | consTProdTProd _ τ1 τ1' τ2 τ2' pCons1 pCons2 =>
     between_TProd
-      (𝓕 A τ1 τ1' pCons1)
-      (𝓕 A τ2 τ2' pCons2)
+      (𝓕 pCons1)
+      (𝓕 pCons2)
   | consTArrowTArrow _ τ1 τ2 τ3 τ4 pCons31 pCons24 =>
     between_TArrow
-      (𝓕 A τ3 τ1 pCons31)
-      (𝓕 A τ2 τ4 pCons24)
+      (𝓕 pCons31)
+      (𝓕 pCons24)
   | consTRecTRecExposeCall _ τl τr pμτlμτrnotA pUnfτlUnfτr =>
     between_TRec
-      (𝓕 ((TRec τl , TRec τr) :: A) τl.[TRec τl/] τr.[TRec τr/] pUnfτlUnfτr)
-  | consTRecTRecUseCall _ τl τr i pμτlμtrinA => (Var i)
+      (𝓕 pUnfτlUnfτr)
+  | consTRecTRecUseCall _ τl τr i pμτlμtrinA => Lam ((Var (S i)) (Var 0))
   end.
+
+Lemma 𝓕_is_value {A} {τi τf} (pC : A ⊢ τi ~ τf) : is_Some $ to_val (𝓕 pC).
+Proof.
+  induction pC; try destruct G; simplify_option_eq; eauto.
+Qed.
+
+Definition 𝓕V {A} {τi τf} (pC : A ⊢ τi ~ τf) : val := is_Some_proj (𝓕_is_value pC).
 
 From fae_gtlc_mu.stlc_mu Require Export typing lang lib.fix.
 
@@ -42,7 +49,7 @@ Definition pair_to_static_function (p : cast_calculus.types.type * cast_calculus
   TArrow <<p.1>> <<p.2>>.
 
 Lemma 𝓕_typed (A : list (cast_calculus.types.type * cast_calculus.types.type)) (τi τf : cast_calculus.types.type) (pτiConsτf : A ⊢ τi ~ τf) :
-  (map pair_to_static_function A) ⊢ₛ (𝓕 A τi τf pτiConsτf) : (<<τi>> → <<τf>>).
+  (map pair_to_static_function A) ⊢ₛ (𝓕 pτiConsτf) : (TArrow <<τi>> <<τf>>).
 Proof.
   induction pτiConsτf; simpl.
   - apply extract_typed.
@@ -68,7 +75,7 @@ Proof.
     rewrite map_cons in IHpτiConsτf.
     repeat rewrite unfolding_backtranslation_commutes in IHpτiConsτf.
     apply IHpτiConsτf.
-  - apply Var_typed.
-    rewrite list_lookup_fmap.
+  - apply Lam_typed. eapply App_typed. apply Var_typed.
+    simpl. rewrite list_lookup_fmap.
     by rewrite pμτlμtrinA.
 Admitted.
