theories/cast_calculus/consistency/equivalent/proof.v
@@ -1,0 +1,7 @@
+From Autosubst Require Export Autosubst.
+From fae_gtlc_mu Require Import prelude.
+From fae_gtlc_mu.cast_calculus Require Import types.
+From fae_gtlc_mu.cast_calculus.consistency Require Import standard structural.definition equivalent.symmetric.
+
+Lemma standard_implies_structural_consistency (τ τ' : type) (Pc : cons_stand 0 τ τ') : [] ⊢ τ ~ τ'.
+Admitted.
