theories/refinements/prelude.v
@@ -1,0 +1,43 @@
+From iris.algebra Require Export base.
+From iris.base_logic Require Import upred.
+From iris.program_logic Require Import weakestpre.
+From iris.base_logic Require Import invariants.
+From Autosubst Require Export Autosubst.
+Import uPred.
+
+Canonical Structure varO := leibnizO var.
+
+Section Autosubst_Lemmas.
+  Context {term : Type} {Ids_term : Ids term}
+          {Rename_term : Rename term} {Subst_term : Subst term}
+          {SubstLemmas_term : SubstLemmas term}.
+
+  Lemma iter_up (m x : nat) (f : var → term) :
+    upn m f x = if lt_dec x m then ids x else rename (+m) (f (x - m)).
+  Proof.
+    revert x; induction m as [|m IH]=> -[|x];
+      repeat (destruct (lt_dec _ _) || asimpl || rewrite IH); auto with lia.
+  Qed.
+End Autosubst_Lemmas.
+
+Ltac properness :=
+  repeat match goal with
+  | |- (∃ _: _, _)%I ≡ (∃ _: _, _)%I => apply exist_proper =>?
+  | |- (∀ _: _, _)%I ≡ (∀ _: _, _)%I => apply forall_proper =>?
+  | |- (_ ∧ _)%I ≡ (_ ∧ _)%I => apply and_proper
+  | |- (_ ∨ _)%I ≡ (_ ∨ _)%I => apply or_proper
+  | |- (_ → _)%I ≡ (_ → _)%I => apply impl_proper
+  | |- (WP _ {{ _ }})%I ≡ (WP _ {{ _ }})%I => apply wp_proper =>?
+  | |- (▷ _)%I ≡ (▷ _)%I => apply later_proper
+  | |- (□ _)%I ≡ (□ _)%I => apply intuitionistically_proper
+  | |- (_ ∗ _)%I ≡ (_ ∗ _)%I => apply sep_proper
+  | |- (inv _ _)%I ≡ (inv _ _)%I => apply (contractive_proper _)
+  end.
+
+Ltac solve_proper_alt :=
+  repeat intro; (simpl + idtac);
+  by repeat match goal with H : _ ≡{_}≡ _|- _ => rewrite H end.
+
+Reserved Notation "⟦ τ ⟧" (at level 0, τ at level 70).
+Reserved Notation "⟦ τ ⟧ₑ" (at level 0, τ at level 70).
+Reserved Notation "⟦ Γ ⟧*" (at level 0, Γ at level 70).
