theories/refinements/static_gradual/compat_easy.v
@@ -1,0 +1,251 @@
+From fae_gtlc_mu.refinements.static_gradual Require Export rules_binary logrel_binary.
+From fae_gtlc_mu.cast_calculus Require Export types typing.
+From fae_gtlc_mu.stlc_mu Require Export lang.
+From fae_gtlc_mu.cast_calculus Require Export lang.
+From fae_gtlc_mu.cast_calculus Require Export lang.
+From iris.algebra Require Import list.
+From iris.proofmode Require Import tactics.
+From iris.program_logic Require Import lifting.
+
+Section bin_log_def.
+  Context `{!heapG Σ, !gradRN Σ}.
+  Notation D := (prodO stlc_mu.lang.valO cast_calculus.lang.valO -n> iProp Σ).
+
+  Definition bin_log_related
+  (Γ : list cast_calculus.types.type) (e : stlc_mu.lang.expr) (e' : cast_calculus.lang.expr) (τ : cast_calculus.types.type) :=
+    ∀ Δ vvs (ei' : cast_calculus.lang.expr), env_Persistent Δ →
+    initially_inv ei' ∗ ⟦ Γ ⟧* Δ vvs ⊢
+    ⟦ τ ⟧ₑ Δ (e.[stlc_mu.typing.env_subst (vvs.*1)], e'.[cast_calculus.typing.env_subst (vvs.*2)]).
+End bin_log_def.
+
+Notation "Γ ⊨ e '≤log≤' e' : τ" :=
+  (bin_log_related Γ e e' τ) (at level 74, e, e', τ at next level).
+
+Section fundamental.
+  Context `{!heapG Σ,!gradRN Σ}.
+  Notation D := (prodO stlc_mu.lang.valO cast_calculus.lang.valO -n> iPropO Σ).
+  (* Implicit Types e : stlc_mu.lang.expr. *)
+  Local Hint Resolve to_of_val : core.
+
+  Local Tactic Notation "smart_wp_bind" uconstr(ctx) ident(v) ident(w)
+        constr(Hv) uconstr(Hp) :=
+    iApply (wp_bind (fill [ctx]));
+    iApply (wp_wand with "[-]");
+      [iApply Hp; iFrame "#"; trivial|];
+    iIntros (v); iDestruct 1 as (w) Hv.
+
+  (* Put all quantifiers at the outer level *)
+  Lemma bin_log_related_alt {Γ e e' τ} : Γ ⊨ e ≤log≤ e' : τ → ∀ Δ vvs ei' K',
+    env_Persistent Δ →
+    initially_inv ei' ∗ ⟦ Γ ⟧* Δ vvs ∗ currently_half (fill K' (e'.[cast_calculus.typing.env_subst (vvs.*2)]))
+    ⊢ WP e.[stlc_mu.typing.env_subst (vvs.*1)] {{ v, ∃ v',
+        currently_half (fill K' (cast_calculus.lang.of_val v')) ∗ interp τ Δ (v, v') }}.
+  Proof.
+    iIntros (Hlog Δ vvs K ρ ?) "[#Hρ [HΓ Hj]]". asimpl.
+    iApply (Hlog with "[HΓ]"); iFrame. eauto.
+  Qed.
+
+  Notation "'` H" := (bin_log_related_alt H) (at level 8).
+
+  Lemma bin_log_related_var Γ x τ :
+    Γ !! x = Some τ → Γ ⊨ stlc_mu.lang.Var x ≤log≤ cast_calculus.lang.Var x : τ.
+  Proof.
+    iIntros (? Δ vvs ρ ?) "[#Hρ #HΓ]". iIntros (K) "Hj /=".
+    iDestruct (interp_env_Some_l with "HΓ") as ([v v']) "[Heq Hv]"; first done.
+    iDestruct "Heq" as %Heq.
+    erewrite !stlc_mu.typing.env_subst_lookup; rewrite ?list_lookup_fmap ?Heq; eauto.
+    erewrite !cast_calculus.typing.env_subst_lookup; rewrite ?list_lookup_fmap ?Heq; eauto.
+    iApply wp_value. eauto.
+  Qed.
+
+  Lemma bin_log_related_unit Γ : Γ ⊨ stlc_mu.lang.Unit ≤log≤ cast_calculus.lang.Unit : TUnit.
+  Proof.
+    iIntros (Δ vvs ρ ?) "#[Hρ HΓ]". iIntros (K) "Hj /=".
+    iApply wp_value. iExists UnitV; eauto.
+  Qed.
+
+  Lemma bin_log_related_pair Γ e1 e2 e1' e2' τ1 τ2
+      (IHHtyped1 : Γ ⊨ e1 ≤log≤ e1' : τ1)
+      (IHHtyped2 : Γ ⊨ e2 ≤log≤ e2' : τ2) :
+    Γ ⊨ stlc_mu.lang.Pair e1 e2 ≤log≤ Pair e1' e2' : TProd τ1 τ2.
+  Proof.
+    iIntros (Δ vvs ρ ?) "#[Hρ HΓ]"; iIntros (K) "Hj /=".
+    smart_wp_bind (stlc_mu.lang.PairLCtx e2.[stlc_mu.typing.env_subst _]) v v' "[Hv #Hiv]"
+      ('`IHHtyped1 _ _ _ ((PairLCtx e2'.[env_subst _]) :: K)).
+    smart_wp_bind (stlc_mu.lang.PairRCtx v) w w' "[Hw #Hiw]"
+      ('`IHHtyped2 _ _ _ ((PairRCtx v') :: K)).
+    iApply wp_value.
+    iExists (PairV v' w'); iFrame "Hw".
+    iExists (v, v'), (w, w'); simpl; repeat iSplit; trivial.
+  Qed.
+
+  Lemma bin_log_related_fst Γ e e' τ1 τ2
+      (IHHtyped : Γ ⊨ e ≤log≤ e' : TProd τ1 τ2) :
+    Γ ⊨ stlc_mu.lang.Fst e ≤log≤ Fst e' : τ1.
+  Proof.
+    iIntros (Δ vvs ρ ?) "[#Hρ #HΓ]"; iIntros (K) "Hj /=".
+    smart_wp_bind (stlc_mu.lang.FstCtx) v v' "[Hv #Hiv]" ('`IHHtyped _ _ _ (FstCtx :: K)); cbn.
+    iDestruct "Hiv" as ([w1 w1'] [w2 w2']) "#[% [Hw1 Hw2]]"; simplify_eq.
+    iMod (step_fst _ _ K (of_val w1') (of_val w2') with "[-]") as "Hw"; eauto.
+    iApply wp_pure_step_later; auto. iApply wp_value; auto.
+  Qed.
+
+  Lemma bin_log_related_snd Γ e e' τ1 τ2
+      (IHHtyped : Γ ⊨ e ≤log≤ e' : TProd τ1 τ2) :
+    Γ ⊨ stlc_mu.lang.Snd e ≤log≤ Snd e' : τ2.
+  Proof.
+    iIntros (Δ vvs ρ ?) "#[Hρ HΓ]"; iIntros (K) "Hj /=".
+    smart_wp_bind (stlc_mu.lang.SndCtx) v v' "[Hv #Hiv]" ('`IHHtyped _ _ _ (SndCtx :: K)); cbn.
+    iDestruct "Hiv" as ([w1 w1'] [w2 w2']) "#[% [Hw1 Hw2]]"; simplify_eq.
+    iMod (step_snd _ _ K (of_val w1') (of_val w2') with "[-]") as "Hw"; eauto.
+    iApply wp_pure_step_later; auto. iApply wp_value; auto.
+  Qed.
+
+  Lemma bin_log_related_injl Γ e e' τ1 τ2
+      (IHHtyped : Γ ⊨ e ≤log≤ e' : τ1) :
+    Γ ⊨ stlc_mu.lang.InjL e ≤log≤ InjL e' : (TSum τ1 τ2).
+  Proof.
+    iIntros (Δ vvs ρ ?) "#[Hρ HΓ]"; iIntros (K) "Hj /=".
+    smart_wp_bind (stlc_mu.lang.InjLCtx) v v' "[Hv #Hiv]"
+      ('`IHHtyped _ _ _ (InjLCtx :: K)); cbn.
+    iApply wp_value. repeat rewrite /= to_of_val. eauto.
+    iExists (InjLV v'); iFrame "Hv".
+    iLeft; iExists (_,_); eauto 10.
+  Qed.
+
+  Lemma bin_log_related_injr Γ e e' τ1 τ2
+      (IHHtyped : Γ ⊨ e ≤log≤ e' : τ2) :
+    Γ ⊨ stlc_mu.lang.InjR e ≤log≤ InjR e' : TSum τ1 τ2.
+  Proof.
+    iIntros (Δ vvs ρ ?) "#[Hρ HΓ]"; iIntros (K) "Hj /=".
+    smart_wp_bind (stlc_mu.lang.InjRCtx) v v' "[Hv #Hiv]"
+      ('`IHHtyped _ _ _ (InjRCtx :: K)); cbn.
+    iApply wp_value. repeat rewrite /= to_of_val. eauto.
+    iExists (InjRV v'); iFrame "Hv".
+    iRight; iExists (_,_); eauto 10.
+  Qed.
+
+  Lemma bin_log_related_case Γ (e0 e1 e2 : stlc_mu.lang.expr) (e0' e1' e2' : cast_calculus.lang.expr) τ1 τ2 τ3
+      (Hclosed2 : ∀ f, e1.[upn (S (length Γ)) f] = e1)
+      (Hclosed3 : ∀ f, e2.[upn (S (length Γ)) f] = e2)
+      (Hclosed2' : ∀ f, e1'.[upn (S (length Γ)) f] = e1')
+      (Hclosed3' : ∀ f, e2'.[upn (S (length Γ)) f] = e2')
+      (IHHtyped1 : Γ ⊨ e0 ≤log≤ e0' : TSum τ1 τ2)
+      (IHHtyped2 : τ1 :: Γ ⊨ e1 ≤log≤ e1' : τ3)
+      (IHHtyped3 : τ2 :: Γ ⊨ e2 ≤log≤ e2' : τ3) :
+    Γ ⊨ stlc_mu.lang.Case e0 e1 e2 ≤log≤ Case e0' e1' e2' : τ3.
+  Proof.
+    iIntros (Δ vvs ρ ?) "#[Hρ HΓ]"; iIntros (K) "Hj /=".
+    iDestruct (interp_env_length with "HΓ") as %?.
+    smart_wp_bind (stlc_mu.lang.CaseCtx _ _) v v' "[Hv #Hiv]"
+      ('`IHHtyped1 _ _ _ ((CaseCtx _ _) :: K)); cbn.
+    iDestruct "Hiv" as "[Hiv|Hiv]".
+    - iDestruct "Hiv" as ([w w']) "[% Hw]"; simplify_eq.
+      iMod (step_case_inl _ _ K (of_val w') with "[-]") as "Hz"; eauto.
+      simpl.
+      iApply wp_pure_step_later; auto 1 using to_of_val. iNext.
+      asimpl. iApply ('`IHHtyped2 _ ((w,w') :: vvs)); repeat iSplit; eauto.
+      iApply interp_env_cons; auto.
+    - iDestruct "Hiv" as ([w w']) "[% Hw]"; simplify_eq.
+      iMod (step_case_inr _ _ K (of_val w') with "[-]") as "Hz"; eauto.
+      simpl.
+      iApply wp_pure_step_later; auto 1 using to_of_val. iNext.
+      asimpl. iApply ('`IHHtyped3 _ ((w,w') :: vvs)); repeat iSplit; eauto.
+      iApply interp_env_cons; auto.
+  Qed.
+
+  Lemma bin_log_related_lam Γ (e : stlc_mu.lang.expr) (e' : cast_calculus.lang.expr) τ1 τ2
+      (Hclosed : ∀ f, e.[upn (S (length Γ)) f] = e)
+      (Hclosed' : ∀ f, e'.[upn (S (length Γ)) f] = e')
+      (IHHtyped : τ1 :: Γ ⊨ e ≤log≤ e' : τ2) :
+    Γ ⊨ stlc_mu.lang.Lam e ≤log≤ Lam e' : TArrow τ1 τ2.
+  Proof.
+    iIntros (Δ vvs ρ ?) "#[Hρ HΓ]"; iIntros (K) "Hj /=".
+    iApply wp_value. iExists (LamV _). iIntros "{$Hj} !#".
+    iIntros ([v v']) "#Hiv". iIntros (K') "Hj".
+    iDestruct (interp_env_length with "HΓ") as %?.
+    iApply wp_pure_step_later; auto 1 using to_of_val. iNext.
+    iMod (step_lam _ _ K' _ (of_val v') with "[-]") as "Hz"; eauto.
+    asimpl. iApply ('`IHHtyped _ ((v,v') :: vvs)); repeat iSplit; eauto.
+    iApply interp_env_cons; iSplit; auto.
+  Qed.
+
+  Lemma bin_log_related_app Γ e1 e2 e1' e2' τ1 τ2
+      (IHHtyped1 : Γ ⊨ e1 ≤log≤ e1' : TArrow τ1 τ2)
+      (IHHtyped2 : Γ ⊨ e2 ≤log≤ e2' : τ1) :
+    Γ ⊨ stlc_mu.lang.App e1 e2 ≤log≤ App e1' e2' :  τ2.
+  Proof.
+    iIntros (Δ vvs ρ ?) "#[Hρ HΓ]"; iIntros (K) "Hj /=".
+    smart_wp_bind (stlc_mu.lang.AppLCtx (e2.[stlc_mu.typing.env_subst (vvs.*1)])) v v' "[Hv #Hiv]"
+      ('`IHHtyped1 _ _ _ (((AppLCtx (e2'.[env_subst (vvs.*2)]))) :: K)); cbn.
+    smart_wp_bind (stlc_mu.lang.AppRCtx v) w w' "[Hw #Hiw]"
+                  ('`IHHtyped2 _ _ _ ((AppRCtx v') :: K)); cbn.
+    iApply ("Hiv" $! (w, w') with "Hiw"); simpl; eauto.
+  Qed.
+
+  Lemma bin_log_related_fold Γ e e' τ
+      (IHHtyped : Γ ⊨ e ≤log≤ e' : τ.[(TRec τ)/]) :
+    Γ ⊨ stlc_mu.lang.Fold e ≤log≤ cast_calculus.lang.Fold e' : TRec τ.
+  Proof.
+    iIntros (Δ vvs ρ ?) "#[Hρ HΓ]"; iIntros (K) "Hj /=".
+    iApply (wp_bind (fill [stlc_mu.lang.FoldCtx])).
+    iApply (wp_wand with "[Hj]"). iApply ('`IHHtyped _ _ _ (FoldCtx :: K)). iFrame. auto.
+    iIntros (v); iDestruct 1 as (v') "[Hv #Hiv]".
+    iApply wp_value.
+    iExists (FoldV v'). iFrame "Hv".
+    rewrite fixpoint_interp_rec1_eq /= -interp_subst.
+    iAlways. iExists (_, _). eauto.
+  Qed.
+
+  (* Theorem binary_fundamental_embedding Γ (e : stlc_mu.lang.expr) τ : *)
+  (*   Γ ⊢ₛ e : τ → Γ ⊨ e ≤log≤ e : τ. *)
+  (* Proof. *)
+  (*   induction 1. *)
+  (*   - by apply bin_log_related_var. *)
+  (*   - by apply bin_log_related_unit. *)
+  (*   - apply bin_log_related_pair; eauto. *)
+  (*   - eapply bin_log_related_fst; eauto. *)
+  (*   - eapply bin_log_related_snd; eauto. *)
+  (*   - eapply bin_log_related_injl; eauto. *)
+  (*   - eapply bin_log_related_injr; eauto. *)
+  (*   - eapply bin_log_related_case; eauto; *)
+  (*       match goal with H : _ |- _ => eapply (typed_n_closed _ _ _ H) end. *)
+  (*   - eapply bin_log_related_lam; eauto; *)
+  (*       match goal with H : _ |- _ => eapply (typed_n_closed _ _ _ H) end. *)
+  (*   - eapply bin_log_related_app; eauto. *)
+  (*   - eapply bin_log_related_tlam; eauto with typeclass_instances. *)
+  (*   - eapply bin_log_related_tapp; eauto. *)
+  (*   - eapply bin_log_related_fold; eauto. *)
+  (*   - eapply bin_log_related_unfold; eauto. *)
+  (*   - eapply bin_log_related_alloc; eauto. *)
+  (*   - eapply bin_log_related_load; eauto. *)
+  (*   - eapply bin_log_related_store; eauto. *)
+  (* Qed. *)
+
+  (* Theorem binary_fundamental_embedding Γ e τ : *)
+  (*   Γ ⊢ₜ e : τ → Γ ⊨ e ≤log≤ e : τ. *)
+  (* Proof. *)
+  (*   induction 1. *)
+  (*   - by apply bin_log_related_var. *)
+  (*   - by apply bin_log_related_unit. *)
+  (*   - apply bin_log_related_pair; eauto. *)
+  (*   - eapply bin_log_related_fst; eauto. *)
+  (*   - eapply bin_log_related_snd; eauto. *)
+  (*   - eapply bin_log_related_injl; eauto. *)
+  (*   - eapply bin_log_related_injr; eauto. *)
+  (*   - eapply bin_log_related_case; eauto; *)
+  (*       match goal with H : _ |- _ => eapply (typed_n_closed _ _ _ H) end. *)
+  (*   - eapply bin_log_related_lam; eauto; *)
+  (*       match goal with H : _ |- _ => eapply (typed_n_closed _ _ _ H) end. *)
+  (*   - eapply bin_log_related_app; eauto. *)
+  (*   - eapply bin_log_related_tlam; eauto with typeclass_instances. *)
+  (*   - eapply bin_log_related_tapp; eauto. *)
+  (*   - eapply bin_log_related_fold; eauto. *)
+  (*   - eapply bin_log_related_unfold; eauto. *)
+  (*   - eapply bin_log_related_alloc; eauto. *)
+  (*   - eapply bin_log_related_load; eauto. *)
+  (*   - eapply bin_log_related_store; eauto. *)
+  (* Qed. *)
+
+
+End fundamental.
