theories/refinements/static_gradual/logrel_binary.v
@@ -1,0 +1,365 @@
+From iris.proofmode Require Import tactics.
+From iris.program_logic Require Export weakestpre.
+From iris.base_logic Require Export invariants.
+From fae_gtlc_mu.backtranslation.cast_help Require Export embed.
+From fae_gtlc_mu.refinements Require Export prelude.
+From fae_gtlc_mu.refinements.static_gradual Require Export rules_binary.
+From fae_gtlc_mu.cast_calculus Require Export types.
+From iris.algebra Require Import list.
+From stdpp Require Import tactics.
+Import uPred.
+
+(* Definition exprO := stlc_mu.lang.expr. *)
+(* Definition exprO' := cast_calculus.lang.expr. *)
+
+(* Definition valO := stlc_mu.lang.valO. *)
+(* Definition valO' := cast_calculus.lang.valO'. *)
+
+(* HACK: move somewhere else *)
+Ltac auto_equiv :=
+  (* Deal with "pointwise_relation" *)
+  repeat lazymatch goal with
+  | |- pointwise_relation _ _ _ _ => intros ?
+  end;
+  (* Normalize away equalities. *)
+  repeat match goal with
+  | H : _ ≡{_}≡ _ |-  _ => apply (discrete_iff _ _) in H
+  | _ => progress simplify_eq
+  end;
+  (* repeatedly apply congruence lemmas and use the equalities in the hypotheses. *)
+  try (f_equiv; fast_done || auto_equiv).
+
+Definition logN : namespace := nroot .@ "logN".
+
+(** interp : is a binary logical relation. *)
+Section logrel.
+  Context `{!heapG Σ, !gradRN Σ}.
+  Notation D := (prodO stlc_mu.lang.valO cast_calculus.lang.valO -n> iPropO Σ).
+  Implicit Types τi : D.
+  Implicit Types Δ : listO D.
+  (* Implicit Types interp : listO D → D. *)
+  Notation RelV := (listO D -n> D). (* value relation on (open) types *)
+
+  (* we get Initially from definition in fundamental_binary *)
+
+  Definition interp_expr (interp_cor_val : RelV) (Δ : listO D)
+      (ee : stlc_mu.lang.expr * cast_calculus.lang.expr) : iProp Σ := (∀ K',
+    currently_half (fill K' (ee.2)) →
+    WP ee.1 {{ v, ∃ v', currently_half (fill K' (of_val v')) ∗ interp_cor_val Δ (v, v') }})%I.
+  Global Instance interp_expr_ne n :
+    Proper (dist n ==> dist n ==> (=) ==> dist n) interp_expr.
+  Proof. solve_proper. Qed.
+
+  Program Definition ctx_lookup (x : var) : RelV := λne Δ,
+    from_option id (cconst True)%I (Δ !! x).
+  (* defaults to something which is trivially true if not in scope; OK, this will never happen in actual type derivations *)
+  Solve Obligations with solve_proper.
+
+  (** For the recursive call to structurally smaller types,
+      we will use the names interp, interp1, interp2... *)
+
+  Program Definition interp_unit : RelV := λne Δ ww,
+    (⌜ww.1 = stlc_mu.lang.UnitV⌝ ∧ ⌜ww.2 = cast_calculus.lang.UnitV⌝)%I.
+  Solve Obligations with solve_proper_alt.
+
+  Program Definition interp_sum
+      (interp1 interp2 : RelV) : RelV := λne Δ ww,
+    ((∃ vv', ⌜ww = (stlc_mu.lang.InjLV (vv'.1), InjLV (vv'.2))⌝ ∧ interp1 Δ vv') ∨
+     (∃ vv', ⌜ww = (stlc_mu.lang.InjRV (vv'.1), InjRV (vv'.2))⌝ ∧ interp2 Δ vv'))%I.
+  Solve Obligations with repeat intros ?; simpl; auto_equiv.
+
+  Program Definition interp_prod
+      (interp1 interp2 : RelV) : RelV := λne Δ ww,
+    (∃ v1v1' v2v2', ⌜ww = (stlc_mu.lang.PairV (v1v1'.1) (v2v2'.1), cast_calculus.lang.PairV (v1v1'.2) (v2v2'.2))⌝ ∧
+                interp1 Δ v1v1' ∧ interp2 Δ v2v2')%I.
+  Solve Obligations with repeat intros ?; simpl; auto_equiv.
+
+  Program Definition interp_arrow
+      (interp1 interp2 : RelV) : RelV := λne Δ ww,
+    (□ ∀ vv, interp1 Δ vv →
+             interp_expr
+               interp2 Δ (stlc_mu.lang.App (stlc_mu.lang.of_val (ww.1)) (stlc_mu.lang.of_val (vv.1)),
+                          cast_calculus.lang.App (cast_calculus.lang.of_val (ww.2)) (cast_calculus.lang.of_val (vv.2))))%I.
+  Solve Obligations with repeat intros ?; simpl; auto_equiv.
+
+  Program Definition interp_rec1 (* interp_rec1 interp Δ : D → D *)
+      (interp : RelV) (Δ : listO D) (μ : D) : D := λne ww,
+    (□ ∃ vv, ⌜ww = (stlc_mu.lang.FoldV (vv.1), cast_calculus.lang.FoldV (vv.2))⌝ ∧ ▷ interp (μ :: Δ) vv)%I.
+  Solve Obligations with repeat intros ?; simpl; auto_equiv.
+
+  Global Instance interp_rec1_contractive
+    (interp : listO D -n> D) (Δ : listO D) : Contractive (interp_rec1 interp Δ).
+  Proof. by solve_contractive. Qed.
+
+  Lemma fixpoint_interp_rec1_eq (interp : RelV) Δ x :
+    fixpoint (interp_rec1 interp Δ) x ≡ interp_rec1 interp Δ (fixpoint (interp_rec1 interp Δ)) x.
+  Proof. exact: (fixpoint_unfold (interp_rec1 interp Δ) x). Qed.
+
+  (* Definition interp_rec (interp : RelV) Δ : D := *)
+  (*   fixpoint (interp_rec1 interp Δ). *)
+
+  (* Global Instance interp_rec_ne n : Proper (dist (A := RelV) n ==> dist (A := RelV) n) interp_rec. *)
+
+
+  Program Definition interp_rec (interp : RelV) : RelV := λne Δ,
+    fixpoint (interp_rec1 interp Δ).
+  Next Obligation.
+    intros interp n Δ1 Δ2 HΔ; apply fixpoint_ne => τi ww. solve_proper.
+  Qed.
+
+  Global Instance interp_rec_ne n : Proper (dist n ==> dist n) interp_rec.
+  Proof.
+    repeat intros ?.
+    rewrite /interp_rec /=. apply (fixpoint_ne (interp_rec1 _ _)).
+    repeat intros ?. unfold interp_rec1.
+    simpl.
+    auto_equiv.
+  Qed.
+
+  (* Unset Printing Notations. *)
+  (* Set Printing Implicit. *)
+  (* Set Printing Notations. *)
+  (* Set Printing Coercions. *)
+
+  (* Unset Printing Notations. *)
+
+
+  (* Set Printing Implicit. *)
+  (* Unset Printing Implicit. *)
+
+  (* Set Printing All. *)
+
+  Definition castupV_TUnit (v : val) : val :=
+    (CastV v TUnit ⋆ (From_ground_to_unknown _ Ground_TUnit)).
+
+  Definition castupV_TSum (v : val) : val :=
+    (CastV v (TSum ⋆ ⋆) ⋆ (From_ground_to_unknown _ Ground_TSum)).
+
+  Definition castupV_TProd (v : val) : val :=
+    (CastV v (TProd ⋆ ⋆) ⋆ (From_ground_to_unknown _ Ground_TProd)).
+
+  Definition castupV_TArrow (v : val) : val :=
+    (CastV v (TArrow ⋆ ⋆) ⋆ (From_ground_to_unknown _ Ground_TArrow)).
+
+  Definition castupV_TRec (v : val) : val :=
+    (CastV v (TRec ⋆) ⋆ (From_ground_to_unknown _ Ground_TRec)).
+
+  (* interp_unknown1 : RelV -n> RelV *)
+  (* Program Definition interp_unknown1 : RelV -n> RelV := λne μR Δ ww', *)
+  Program Definition interp_unknown1 : RelV -n> RelV := λne μR Δ ww',
+    (□ (
+      (∃ vv', ⌜ ww' = (embedV_TUnit (vv'.1) , castupV_TUnit vv'.2) ⌝ ∧
+              ▷ interp_unit Δ vv' )
+    ∨ (∃ pp', ⌜ ww' = (embedV_Ground_TProd (pp'.1) , castupV_TProd pp'.2) ⌝ ∧
+              ▷ interp_prod μR μR Δ pp')
+    ∨ (∃ ss', ⌜ ww' = (embedV_Ground_TSum (ss'.1) , castupV_TSum ss'.2) ⌝ ∧
+              ▷ interp_sum μR μR Δ ss' )
+    ∨ (∃ ff', ⌜ ww' = (embedV_Ground_TArrow (ff'.1) , castupV_TArrow ff'.2) ⌝ ∧
+              ▷ interp_arrow μR μR Δ ff' )
+    ∨ (∃ ur', ⌜ ww' = (stlc_mu.lang.FoldV (stlc_mu.lang.InjRV (ur'.1)) , castupV_TRec ur'.2) ⌝ ∧
+              ▷ interp_rec μR Δ (stlc_mu.lang.FoldV ur'.1 , ur'.2))
+    ))%I.
+  Next Obligation.
+    repeat intros ?; simpl; auto_equiv.
+  Qed.
+  Next Obligation.
+    repeat intros ?.  simpl; auto_equiv.
+    change (interp_rec μR x ≡{n}≡ interp_rec μR y). (*note*)
+    by f_equiv.
+  Qed.
+  Next Obligation.
+    repeat intros ?; simpl; auto_equiv.
+    change (interp_rec x x0 ≡{n}≡ interp_rec y x0). (*not use autogenerated names*)
+    f_equiv. by f_equiv.
+  Qed.
+
+  Typeclasses Opaque interp_rec.
+
+  Arguments interp_rec _ : simpl never.
+
+  Global Instance interp_unknown1_contractive : Contractive (interp_unknown1).
+  Proof.
+    repeat intros ?.
+    unfold interp_unknown1.
+    simpl. do 1 f_equiv.
+    repeat (f_equiv; first solve_contractive).
+    f_equiv. simpl. repeat intros ?.
+    f_equiv. f_equiv. intros ?. f_equiv. apply later_contractive.
+    destruct n; first done.
+    simpl in *. f_equiv.
+    intros ?. f_equiv. intros ?. by repeat f_equiv.
+
+    f_equiv. f_equiv. intros ?. f_equiv. apply later_contractive. destruct n; first done. simpl in *. by repeat f_equiv.
+    f_equiv. f_equiv. intros ?. f_equiv. apply later_contractive. destruct n; first done. simpl in *. by repeat f_equiv.
+    f_equiv. intros ?. f_equiv. apply later_contractive. destruct n; first done. simpl in *.
+    f_equiv.
+    change (interp_rec x x0 ≡{n}≡ interp_rec y x0). (*not use autogenerated names*)
+    by do 2 f_equiv.
+  Qed.
+
+  (* Global Instance interp_unknown1_contractive : Contractive (interp_unknown1). *)
+  (* Proof. *)
+  (*   repeat intros ?. *)
+  (*   unfold interp_unknown1. *)
+  (*   simpl. do 1 f_equiv. *)
+  (*   repeat (f_equiv; first solve_contractive). *)
+  (*   f_equiv. simpl. repeat intros ?. *)
+  (*   f_equiv. apply later_contractive. *)
+  (*   destruct n; first done. *)
+  (*   simpl in *. f_equiv. *)
+  (*   change (interp_rec x x0 ≡{n}≡ interp_rec y x0). (*not use autogenerated names*) *)
+  (*   by do 2 f_equiv. *)
+  (* Qed. *)
+
+  Definition interp_unknown : listO D -n> D := fixpoint (interp_unknown1).
+
+  Lemma interp_unknown_unfold Δ vv : interp_unknown Δ vv ≡ interp_unknown1 (fixpoint interp_unknown1) Δ vv.
+  Proof.
+    f_equiv.
+    f_equiv.
+    apply fixpoint_unfold.
+  Qed.
+
+  Lemma interp_unknown_unfold' Δ : interp_unknown Δ ≡ interp_unknown1 (fixpoint interp_unknown1) Δ.
+  Proof.
+    f_equiv.
+    apply fixpoint_unfold.
+  Qed.
+
+  Fixpoint interp (τ : cast_calculus.types.type) : listO D -n> D :=
+    match τ return _ with
+    | TUnit => interp_unit
+    | TProd τ1 τ2 => interp_prod (interp τ1) (interp τ2)
+    | TSum τ1 τ2 => interp_sum (interp τ1) (interp τ2)
+    | TArrow τ1 τ2 => interp_arrow (interp τ1) (interp τ2)
+    | TVar x => ctx_lookup x
+    | TRec τ' => interp_rec (interp τ')
+    | TUnknown => interp_unknown
+    end.
+  Notation "⟦ τ ⟧" := (interp τ). (** the actual relations on expressions *)
+
+  Definition interp_env (Γ : list type)
+      (Δ : listO D) (vvs : list (stlc_mu.lang.val * cast_calculus.lang.val)) : iProp Σ :=
+    (⌜length Γ = length vvs⌝ ∗ [∗] zip_with (λ τ, ⟦ τ ⟧ Δ) Γ vvs)%I.
+  Notation "⟦ Γ ⟧*" := (interp_env Γ).
+
+  Class env_Persistent Δ :=
+    ctx_persistentP : Forall (λ τi, ∀ vv, Persistent (τi vv)) Δ.
+  Global Instance ctx_persistent_nil : env_Persistent [].
+  Proof. by constructor. Qed.
+  Global Instance ctx_persistent_cons τi Δ :
+    (∀ vv, Persistent (τi vv)) → env_Persistent Δ → env_Persistent (τi :: Δ).
+  Proof. by constructor. Qed.
+  Global Instance ctx_persistent_lookup Δ x vv :
+    env_Persistent Δ → Persistent (ctx_lookup x Δ vv).
+  Proof. intros HΔ; revert x; induction HΔ=>-[|?] /=; apply _. Qed.
+  Global Instance interp_persistent τ Δ vv :
+    env_Persistent Δ → Persistent (⟦ τ ⟧ Δ vv).
+  Proof.
+    revert vv Δ; induction τ=> vv Δ HΔ; simpl; try apply _.
+    - rewrite /Persistent fixpoint_interp_rec1_eq.
+      rewrite /interp_rec1.
+      rewrite /= intuitionistically_into_persistently.
+      by apply persistently_intro'.
+    - rewrite /Persistent interp_unknown_unfold /= intuitionistically_into_persistently.
+      by apply persistently_intro'.
+  Qed.
+
+  Global Instance interp_env_base_persistent Δ Γ vs :
+  env_Persistent Δ → TCForall Persistent (zip_with (λ τ, ⟦ τ ⟧ Δ) Γ vs).
+  Proof.
+    intros HΔ. revert vs.
+    induction Γ => vs; simpl; destruct vs; constructor; apply _.
+  Qed.
+  Global Instance interp_env_persistent Γ Δ vvs :
+    env_Persistent Δ → Persistent (⟦ Γ ⟧* Δ vvs) := _.
+
+  Lemma interp_weaken Δ1 Π Δ2 τ :
+    ⟦ τ.[upn (length Δ1) (ren (+ length Π))] ⟧ (Δ1 ++ Π ++ Δ2)
+    ≡ ⟦ τ ⟧ (Δ1 ++ Δ2).
+  Proof.
+    revert Δ1 Π Δ2. induction τ=> Δ1 Π Δ2; simpl; auto.
+    - intros ww; simpl; properness; auto. by apply IHτ1. by apply IHτ2.
+    - intros ww; simpl; properness; auto. by apply IHτ1. by apply IHτ2.
+    - unfold interp_expr.
+      intros ww; simpl; properness; auto. by apply IHτ1. by apply IHτ2.
+    - apply fixpoint_proper=> τi ww /=.
+      properness; auto. apply (IHτ (_ :: _)).
+    - rewrite iter_up; destruct lt_dec as [Hl | Hl]; simpl.
+      { by rewrite !lookup_app_l. }
+      (* FIXME: Ideally we wouldn't have to do this kinf of surgery. *)
+      change (bi_ofeO (uPredI (iResUR Σ))) with (uPredO (iResUR Σ)).
+      rewrite !lookup_app_r; [|lia ..]. do 2 f_equiv. lia.
+    - repeat rewrite interp_unknown_unfold'.
+      admit.
+      (* - unfold interp_expr. *)
+      (* intros ww; simpl; properness; auto. by apply (IHτ (_ :: _)). *)
+      (* - intros ww; simpl; properness; auto. by apply IHτ. *)
+  Admitted.
+
+  Lemma interp_subst_up Δ1 Δ2 τ τ' :
+    ⟦ τ ⟧ (Δ1 ++ interp τ' Δ2 :: Δ2)
+    ≡ ⟦ τ.[upn (length Δ1) (τ' .: ids)] ⟧ (Δ1 ++ Δ2).
+  Proof.
+    revert Δ1 Δ2; induction τ=> Δ1 Δ2; simpl; auto.
+    - intros ww; simpl; properness; auto. by apply IHτ1. by apply IHτ2.
+    - intros ww; simpl; properness; auto. by apply IHτ1. by apply IHτ2.
+    - unfold interp_expr.
+      intros ww; simpl; properness; auto. by apply IHτ1. by apply IHτ2.
+    - apply fixpoint_proper=> τi ww /=.
+      properness; auto. apply (IHτ (_ :: _)).
+    - rewrite iter_up; destruct lt_dec as [Hl | Hl]; simpl.
+      { by rewrite !lookup_app_l. }
+      (* FIXME: Ideally we wouldn't have to do this kinf of surgery. *)
+      change (bi_ofeO (uPredI (iResUR Σ))) with (uPredO (iResUR Σ)).
+      rewrite !lookup_app_r; [|lia ..].
+      case EQ: (x - length Δ1) => [|n]; simpl.
+      { symmetry. asimpl. apply (interp_weaken [] Δ1 Δ2 τ'). }
+      change (bi_ofeO (uPredI (iResUR Σ))) with (uPredO (iResUR Σ)).
+      rewrite !lookup_app_r; [|lia ..]. do 2 f_equiv. lia.
+    - admit.
+    (* - unfold interp_expr. *)
+      (* intros ww; simpl; properness; auto. apply (IHτ (_ :: _)). *)
+    (* - intros ww; simpl; properness; auto. by apply IHτ. *)
+  Admitted.
+
+  Lemma interp_subst Δ2 τ τ' v : ⟦ τ ⟧ (⟦ τ' ⟧ Δ2 :: Δ2) v ≡ ⟦ τ.[τ'/] ⟧ Δ2 v.
+  Proof. apply (interp_subst_up []). Qed.
+
+  Lemma interp_env_length Δ Γ vvs : bi_entails (⟦ Γ ⟧* Δ vvs) (⌜length Γ = length vvs⌝).
+  Proof. by iIntros "[% ?]". Qed.
+
+  Lemma interp_env_Some_l Δ Γ vvs x τ :
+    Γ !! x = Some τ → bi_entails (⟦ Γ ⟧* Δ vvs) (∃ vv, ⌜vvs !! x = Some vv⌝ ∧ ⟦ τ ⟧ Δ vv).
+  Proof.
+    iIntros (?) "[Hlen HΓ]"; iDestruct "Hlen" as %Hlen.
+    destruct (lookup_lt_is_Some_2 vvs x) as [v Hv].
+    { by rewrite -Hlen; apply lookup_lt_Some with τ. }
+    iExists v; iSplit. done. iApply (big_sepL_elem_of with "HΓ").
+    apply elem_of_list_lookup_2 with x.
+    rewrite lookup_zip_with; by simplify_option_eq.
+  Qed.
+
+  Lemma interp_env_nil Δ : ⟦ [] ⟧* Δ [].
+  Proof. iSplit; simpl; auto. Qed.
+  Lemma interp_env_cons Δ Γ vvs τ vv :
+    ⟦ τ :: Γ ⟧* Δ (vv :: vvs) ⊣⊢ ⟦ τ ⟧ Δ vv ∗ ⟦ Γ ⟧* Δ vvs.
+  Proof.
+    rewrite /interp_env /= (assoc _ (⟦ _ ⟧ _ _)) -(comm _ ⌜_ = _⌝%I) -assoc.
+    by apply sep_proper; [apply pure_proper; lia|].
+  Qed.
+
+  Lemma interp_env_ren Δ (Γ : list type) vvs τi :
+    ⟦ subst (ren (+1)) <$> Γ ⟧* (τi :: Δ) vvs ⊣⊢ ⟦ Γ ⟧* Δ vvs.
+  Proof.
+    apply sep_proper; [apply pure_proper; by rewrite fmap_length|].
+    revert Δ vvs τi; induction Γ=> Δ [|v vs] τi; csimpl; auto.
+    apply sep_proper; auto. apply (interp_weaken [] [τi] Δ).
+  Qed.
+
+End logrel.
+
+Typeclasses Opaque interp_env.
+Notation "⟦ τ ⟧" := (interp τ).
+Notation "⟦ τ ⟧ₑ" := (interp_expr (interp τ)).
+Notation "⟦ Γ ⟧*" := (interp_env Γ).
