theories/refinements/static_gradual/rules_binary.v
@@ -1,0 +1,215 @@
+From iris.algebra Require Import cmra excl auth frac agree gmap list.
+From iris.program_logic Require Import lifting.
+From iris.proofmode Require Import tactics.
+From fae_gtlc_mu.refinements.static_gradual Require Export rules.
+From fae_gtlc_mu.cast_calculus Require Export lang.
+Import uPred.
+
+Definition gradualN := nroot .@ "gradual".
+
+(** The CMRA for the heap of the specification. *)
+
+Canonical Structure exprO := leibnizO expr.
+
+Definition gradR := prodR fracR (agreeR exprO).
+(* Definition cfgUR := prodUR (optionUR (exclR exprO)) (gen_heapUR loc val). *)
+
+(** The CMRA for the thread pool. *)
+Class gradRN Σ := CFGSG { gradR_inG :> inG Σ gradR; grad_name : gname }.
+
+Definition currently `{gradRN Σ} (e : expr) : iProp Σ :=
+  own grad_name ((1%Qp , to_agree e) : gradR).
+
+Definition currently_half `{gradRN Σ} (e : expr) : iProp Σ :=
+  own grad_name (((1 / 2)%Qp , to_agree e) : gradR).
+
+Definition initially_body `{gradRN Σ} (ei' : expr) : iProp Σ :=
+  (∃ e', (currently_half e')
+            ∗ ⌜rtc erased_step ([ei'] , tt) ([e'] , tt)⌝)%I.
+
+Definition initially_inv `{gradRN Σ} `{invG Σ} (ei' : expr) : iProp Σ :=
+  inv gradualN (initially_body ei').
+
+(* Section definitionsS. *)
+  (* Context `{gradRN Σ}. *)
+
+  (* Definition heapS_mapsto (l : loc) (q : Qp) (v: val) : iProp Σ := *)
+    (* own cfg_name (◯ (ε, {[ l := (q, to_agree v) ]})). *)
+
+  (* Definition tpool_mapsto (e: expr) : iProp Σ := *)
+    (* own cfg_name (◯ (Excl' e, ∅)). *)
+
+  (* Global Instance heapS_mapsto_timeless l q v : Timeless (heapS_mapsto l q v). *)
+  (* Proof. apply _. Qed. *)
+(* End definitionsS. *)
+
+(* Typeclasses Opaque heapS_mapsto tpool_mapsto. *)
+
+(* Notation "l ↦ₛ{ q } v" := (heapS_mapsto l q v) *)
+  (* (at level 20, q at level 50, format "l  ↦ₛ{ q }  v") : bi_scope. *)
+(* Notation "l ↦ₛ v" := (heapS_mapsto l 1 v) (at level 20) : bi_scope. *)
+(* Notation "⤇ e" := (tpool_mapsto e) (at level 20) : bi_scope. *)
+
+Section cfg.
+  Context `{!gradRN Σ}.
+  Context `{!invG Σ}.
+  Implicit Types P Q : iProp Σ.
+  Implicit Types Φ : val → iProp Σ.
+  (* Implicit Types σ : state. *)
+  Implicit Types e : expr.
+  Implicit Types v : val.
+
+  Local Hint Resolve to_of_val : core.
+
+  (** Conversion to tpools and back *)
+  Lemma step_insert_no_fork K e σ κ e' σ' :
+    head_step e σ κ e' σ' [] → erased_step ([fill K e], σ) ([fill K e'], σ').
+  Proof. intros Hst. eexists. eapply (step_atomic _ _ _ _ _ _ _ [] [] []); eauto.
+         by apply: Ectx_step'.
+  Qed.
+
+  Local Set Warnings "-notation-overridden".
+  Lemma step_pure E ei' K e1' e2' :
+    (∀ σ, head_step e1' σ [] e2' σ []) →
+    nclose gradualN ⊆ E →
+    initially_inv ei' ∗ currently_half (fill K e1') ={E}=∗ currently_half (fill K e2').
+  Proof.
+    iIntros (??) "[Hinv Hj]".
+    rewrite /initially_inv /initially_body.
+    iInv gradualN as ">Hinit" "Hclose".
+    iDestruct "Hinit" as (ef') "[Hown %]".
+    rewrite /currently_half.
+    iDestruct (own_valid_2 with "Hown Hj") as %cpa.
+    iDestruct (@own_valid_2 with "Hown Hj") as %[aa bb].
+    admit.
+  (*   simpl in bb. *)
+  (*   iDestruct agree_op_inv' with "bb". *)
+
+
+  (*   (* iDestruct agree_op_inv' with  as %HHH. *) *)
+  (*   %agree_op_inv' *)
+  (*   rewrite -pair_op in asf. *)
+  (*   iSimpl in "asf".  *)
+
+  (*   rewrite currently_half. *)
+  (*   iDestruct (@own_valid_2 with "Hown Hj") *)
+  (*     as %[[?%Excl_included%leibniz_equiv _]%prod_included Hvalid]%auth_both_valid; subst. *)
+  (*   iMod (own_update_2 with "Hown Hj") as "[Hown Hj]". *)
+  (*   { by eapply auth_update, prod_local_update_1, option_local_update, *)
+  (*       (exclusive_local_update _ (Excl (fill K e'))). } *)
+  (*   iFrame "Hj". *)
+  (*   iApply "Hclose". iNext. iExists (fill K e'). iExists σ. iFrame. *)
+  (*   iPureIntro. eapply rtc_r, step_insert_no_fork; eauto. *)
+  (* Qed. *)
+  Admitted.
+
+  Lemma step_fst E ei' K e1' e2' :
+    AsVal e1' → AsVal e2' →
+    nclose gradualN ⊆ E →
+    initially_inv ei' ∗ currently_half (fill K (Fst (Pair e1' e2'))) ={E}=∗ currently_half (fill K e1').
+  Proof. intros [? <-] [? <-]. apply step_pure => σ; econstructor; eauto. Qed.
+
+  Lemma step_snd E ei' K e1' e2' :
+    AsVal e1' → AsVal e2' → nclose gradualN ⊆ E →
+    initially_inv ei' ∗ currently_half (fill K (Snd (Pair e1' e2'))) ={E}=∗ currently_half (fill K e2').
+  Proof. intros [? <-] [? <-]; apply step_pure => σ; econstructor; eauto. Qed.
+
+  (* Lemma step_alloc E ρ K e v: *)
+  (*   IntoVal e v → nclose specN ⊆ E → *)
+  (*   spec_inv ρ ∗ ⤇ fill K (Alloc e) ={E}=∗ ∃ l, ⤇ fill K (Loc l) ∗ l ↦ₛ v. *)
+  (* Proof. *)
+  (*   iIntros (<- ?) "[#Hinv Hj]". rewrite /spec_ctx /tpool_mapsto. *)
+  (*   iInv specN as ">Hinv'" "Hclose". iDestruct "Hinv'" as (e2 σ) "[Hown %]". *)
+  (*   destruct (exist_fresh (dom (gset positive) σ)) as [l Hl%not_elem_of_dom]. *)
+  (*   iDestruct (own_valid_2 _ with "Hown Hj") *)
+  (*     as %[[?%Excl_included%leibniz_equiv _]%prod_included ?]%auth_both_valid. *)
+  (*   subst. *)
+  (*   iMod (own_update_2 with "Hown Hj") as "[Hown Hj]". *)
+  (*   { by eapply auth_update, prod_local_update_1, option_local_update, *)
+  (*      (exclusive_local_update _ (Excl (fill K (Loc l)))). } *)
+  (*   iMod (own_update with "Hown") as "[Hown Hl]". *)
+  (*   { eapply auth_update_alloc, prod_local_update_2, *)
+  (*       (alloc_singleton_local_update _ l (1%Qp,to_agree v)); last done. *)
+  (*     by apply lookup_to_gen_heap_None. } *)
+  (*   iExists l. rewrite /heapS_mapsto. iFrame "Hj Hl". iApply "Hclose". iNext. *)
+  (*   iExists (fill K (Loc l)), (<[l:=v]>σ). *)
+  (*   rewrite to_gen_heap_insert; last eauto. iFrame. iPureIntro. *)
+  (*   eapply rtc_r, step_insert_no_fork; eauto. econstructor; eauto. *)
+  (* Qed. *)
+
+  (* Lemma step_load E ρ K l q v: *)
+  (*   nclose specN ⊆ E → *)
+  (*   spec_inv ρ ∗ ⤇ fill K (Load (Loc l)) ∗ l ↦ₛ{q} v *)
+  (*   ={E}=∗ ⤇ fill K (of_val v) ∗ l ↦ₛ{q} v. *)
+  (* Proof. *)
+  (*   iIntros (?) "(#Hinv & Hj & Hl)". *)
+  (*   rewrite /spec_ctx /tpool_mapsto /heapS_mapsto. *)
+  (*   iInv specN as ">Hinv'" "Hclose". iDestruct "Hinv'" as (e2 σ) "[Hown %]". *)
+  (*   iDestruct (own_valid_2 _ with "Hown Hj") *)
+  (*     as %[[?%Excl_included%leibniz_equiv _]%prod_included ?]%auth_both_valid. *)
+  (*   subst. *)
+  (*   iDestruct (own_valid_2 with "Hown Hl") *)
+  (*     as %[[_ ?%gen_heap_singleton_included]%prod_included _]%auth_both_valid. *)
+  (*   iMod (own_update_2 with "Hown Hj") as "[Hown Hj]". *)
+  (*   { by eapply auth_update, prod_local_update_1, option_local_update, *)
+  (*       (exclusive_local_update _ (Excl (fill K (of_val v)))). } *)
+  (*   iFrame "Hj Hl". iApply "Hclose". iNext. *)
+  (*   iExists (fill K (of_val v)), σ. *)
+  (*   iFrame. iPureIntro. *)
+  (*   eapply rtc_r, step_insert_no_fork; eauto. econstructor; eauto. *)
+  (* Qed. *)
+
+  (* Lemma step_store E ρ K l v' e v: *)
+  (*   IntoVal e v → nclose specN ⊆ E → *)
+  (*   spec_inv ρ ∗ ⤇ fill K (Store (Loc l) e) ∗ l ↦ₛ v' *)
+  (*   ={E}=∗ ⤇ fill K Unit ∗ l ↦ₛ v. *)
+  (* Proof. *)
+  (*   iIntros (<- ?) "(#Hinv & Hj & Hl)". *)
+  (*   rewrite /spec_ctx /tpool_mapsto /heapS_mapsto. *)
+  (*   iInv specN as ">Hinv'" "Hclose". iDestruct "Hinv'" as (e2 σ) "[Hown %]". *)
+  (*   iDestruct (own_valid_2 _ with "Hown Hj") *)
+  (*     as %[[?%Excl_included%leibniz_equiv _]%prod_included ?]%auth_both_valid. *)
+  (*   subst. *)
+  (*   iDestruct (own_valid_2 _ with "Hown Hl") *)
+  (*     as %[[_ Hl%gen_heap_singleton_included]%prod_included _]%auth_both_valid. *)
+  (*   iMod (own_update_2 with "Hown Hj") as "[Hown Hj]". *)
+  (*   { by eapply auth_update, prod_local_update_1, option_local_update, *)
+  (*       (exclusive_local_update _ (Excl (fill K Unit))). } *)
+  (*   iMod (own_update_2 with "Hown Hl") as "[Hown Hl]". *)
+  (*   { eapply auth_update, prod_local_update_2, singleton_local_update, *)
+  (*       (exclusive_local_update _ (1%Qp, to_agree v)); last done. *)
+  (*     by rewrite /to_gen_heap lookup_fmap Hl. } *)
+  (*   iFrame "Hj Hl". iApply "Hclose". iNext. *)
+  (*   iExists (fill K Unit), (<[l:=v]>σ). *)
+  (*   rewrite to_gen_heap_insert; last eauto. iFrame. iPureIntro. *)
+  (*   eapply rtc_r, step_insert_no_fork; eauto. econstructor; eauto. *)
+  (* Qed. *)
+
+  Lemma step_lam E ei' K e1' e2' :
+    AsVal e2' → nclose gradualN ⊆ E →
+    initially_inv ei' ∗ currently_half (fill K (App (Lam e1') e2'))
+    ={E}=∗ currently_half (fill K (e1'.[e2'/])).
+  Proof. intros [? <-]; apply step_pure => σ; econstructor; eauto. Qed.
+
+  (* Lemma step_tlam E ρ K e : *)
+  (*   nclose specN ⊆ E → *)
+  (*   spec_inv ρ ∗ ⤇ fill K (TApp (TLam e)) ={E}=∗ ⤇ fill K e. *)
+  (* Proof. apply step_pure => σ; econstructor; eauto. Qed. *)
+
+  Lemma step_Fold E ei' K e' :
+    AsVal e' → nclose gradualN ⊆ E →
+    initially_inv ei' ∗ currently_half (fill K (Unfold (Fold e'))) ={E}=∗ currently_half (fill K e').
+  Proof. intros [? <-]; apply step_pure => σ; econstructor; eauto. Qed.
+
+  Lemma step_case_inl E ei' K e0' e1' e2' :
+    AsVal e0' → nclose gradualN ⊆ E →
+    initially_inv ei' ∗ currently_half (fill K (Case (InjL e0') e1' e2'))
+      ={E}=∗ currently_half (fill K (e1'.[e0'/])).
+  Proof. intros [? <-]; apply step_pure => σ; econstructor; eauto. Qed.
+
+  Lemma step_case_inr E ei' K e0' e1' e2' :
+    AsVal e0' → nclose gradualN ⊆ E →
+    initially_inv ei' ∗ currently_half (fill K (Case (InjR e0') e1' e2'))
+      ={E}=∗ currently_half (fill K (e2'.[e0'/])).
+  Proof. intros [? <-]; apply step_pure => σ; econstructor; eauto. Qed.
+End cfg.
