theories/stlc_mu/lib/fix.v
@@ -2,7 +2,7 @@ From fae_gtlc_mu Require Export stlc_mu.lang.
 From fae_gtlc_mu Require Export stlc_mu.typing.
 
 Coercion App : expr >-> Funclass.
-Infix "→" := TArrow : type_scope.
+(* Infix "→" := TArrow : type_scope. *)
 
 Definition Fix : expr :=
   Lam (
@@ -10,22 +10,22 @@ Definition Fix : expr :=
         (Fold (Lam (Var 1 ((Unfold (Var 0)) (Var 0)))))
   ).
 
-Definition Fix_typed Γ τ : (Is_Closed τ) -> (Γ ⊢ₛ Fix : ((τ → τ) → τ)).
+Definition Fix_typed Γ τ : (Is_Closed τ) -> (Γ ⊢ₛ Fix : (TArrow (TArrow τ τ) τ)).
 Proof.
   intro P.
   apply Lam_typed.
-  apply App_typed with (τ1 := (TRec (TVar 0 → τ))).
+  apply App_typed with (τ1 := (TRec (TArrow (TVar 0) τ))).
   - apply Lam_typed.
     apply App_typed with (τ1 := τ); first by apply Var_typed.
-    apply App_typed with (τ1 := TRec (TVar 0 → τ)).
-    + apply Unfold_typed_help_2 with (τ := (TVar 0 → τ)).
+    apply App_typed with (τ1 := TRec (TArrow (TVar 0) τ)).
+    + apply Unfold_typed_help_2 with (τ := TArrow (TVar 0) τ).
       asimpl. by rewrite P. by apply Var_typed.
     + by apply Var_typed.
   - apply Fold_typed. asimpl. rewrite P.
     apply Lam_typed.
     apply App_typed with (τ1 := τ); first by apply Var_typed.
-    apply App_typed with (τ1 := TRec (TVar 0 → τ)).
-    + apply Unfold_typed_help_2 with (τ := (TVar 0 → τ)).
+    apply App_typed with (τ1 := TRec (TArrow (TVar 0) τ)).
+    + apply Unfold_typed_help_2 with (τ := (TArrow (TVar 0) τ)).
       asimpl. by rewrite P. by apply Var_typed.
     + by apply Var_typed.
 Qed.
